More on advantage. Clean up, document, refactor.

theories/approxis/examples/advantage.v
@@ -3,27 +3,100 @@ From clutch.approxis Require Export bounded_oracle.
 From Coquelicot Require Import Lub.
 Set Default Proof Using "Type*".
 
+Definition pr_dist (X Y : expr)
+  (σ σ' : state) (v : val) : nonnegreal.
+Proof.
+  unshelve econstructor.
+  1: exact (Rabs ( (( lim_exec (X, σ)) v) - (lim_exec (Y, σ') v) )).
+  apply Rabs_pos.
+Defined.
 
-Definition pr_dist (A : val) (G G' : expr)
-  (σ σ' : state) (v : val) :=
-  Rabs ( (( lim_exec (A G, σ)) v) - (lim_exec (A G', σ') v) )%R.
+Fact pr_dist_triangle' X Y Z σ σ' σ'' v :
+  (pr_dist X Z σ σ'' v <= (pr_dist X Y σ σ' v) + (pr_dist Y Z σ' σ'' v))%R.
+Proof.
+  rewrite /pr_dist. etrans. 2: apply Rabs_triang. right. simpl. f_equal. lra.
+Qed.
 
-Definition advantage (A : val) (G G' : expr) :=
-  Lub_Rbar (λ ε : R, ∃ (σ σ' : state) (v : val), pr_dist A G G' σ σ' v = ε)%R.
+Fact pr_dist_triangle X Y Z v ε1 ε2 ε3 :
+  ((∀ σ σ', pr_dist X Y σ σ' v <= ε1) →
+   (∀ σ σ', pr_dist Y Z σ σ' v <= ε2) →
+   (ε1 + ε2 <= ε3) →
+   ∀ σ σ', pr_dist X Z σ σ' v <= ε3)%R.
+Proof.
+  intros. etrans.
+  1: eapply (pr_dist_triangle' _ Y _ _ σ).
+  etrans. 2: eauto.
+  apply Rplus_le_compat => //.
+Qed.
 
-Lemma advantage_uniform (A : val) (G G' : expr) (ε : R) :
-  (∀ (σ σ' : state) (v : val), pr_dist A G G' σ σ' v <= ε)%R ->
-  (Rbar.Rbar_le (advantage A G G') (Rbar.Finite ε)).
+Definition advantage_rbar (X Y : expr) (v : val) :=
+  Lub.Lub_Rbar (λ ε : R, ∃ (σ σ' : state), nonneg (pr_dist X Y σ σ' v) = ε)%R.
+
+Fact advantage_0_1 X Y v : Rbar.Rbar_le (Rbar.Finite 0) (advantage_rbar X Y v) /\
+                           Rbar.Rbar_le (advantage_rbar X Y v) (Rbar.Finite 1).
+Proof.
+  rewrite /advantage_rbar.
+  set (P := (λ ε : R, ∃ σ0 σ'0 : state, nonneg (pr_dist X Y σ0 σ'0 v) = ε)).
+  epose proof (Lub.Lub_Rbar_correct P) as [is_ub least_ub].
+  rewrite /Lub.is_ub_Rbar in is_ub.
+  split.
+Admitted.
+
+Fact advantage_finite X Y v : Rbar.is_finite (advantage_rbar X Y v).
+Proof.
+  destruct (advantage_0_1 X Y v). by eapply (is_finite_bounded).
+Qed.
+
+Definition advantage (X Y : expr) (v : val) : nonnegreal.
+Proof.
+  unshelve econstructor.
+  1: exact (epsilon ((proj1 (Rbar.is_finite_correct (advantage_rbar X Y v))) (advantage_finite _ _ _))).
+  set (h := (proj1 (Rbar.is_finite_correct (advantage_rbar X Y v)) (advantage_finite X Y v))).
+  opose proof (epsilon_correct _ h) as hh. simpl in hh.
+  simpl.
+  eapply (proj1 (rbar_le_rle _ _)).
+  rewrite -hh.
+  apply advantage_0_1.
+Defined.
+
+Fact advantage_ub X Y v : forall σ σ', (pr_dist X Y σ σ' v <= advantage X Y v)%R.
+Proof.
+  intros. rewrite /advantage.
+  set (h := (proj1 (Rbar.is_finite_correct (advantage_rbar X Y v)) (advantage_finite X Y v))).
+  opose proof (epsilon_correct _ h) as hh. simpl in hh.
+  simpl.
+  eapply (proj1 (rbar_le_rle _ _)).
+  rewrite -hh.
+  rewrite /advantage_rbar.
+  set (P := (λ ε : R, ∃ σ0 σ'0 : state, nonneg (pr_dist X Y σ0 σ'0 v) = ε)).
+  epose proof (Lub.Lub_Rbar_correct P) as [is_ub least_ub].
+  rewrite /Lub.is_ub_Rbar in is_ub.
+  apply is_ub.
+  rewrite /P. exists σ, σ'.
+  done.
+Qed.
+
+Lemma advantage_uniform (X Y : expr) v (ε : R) :
+  (∀ (σ σ' : state), pr_dist X Y σ σ' v <= ε)%R ->
+  (Rbar.Rbar_le (advantage_rbar X Y v) (Rbar.Finite ε)).
 Proof.
   intros hε.
-  rewrite /advantage.
-  set (E := (λ ε0 : R, ∃ (σ σ' : state) (v : val), pr_dist A G G' σ σ' v = ε0)).
-  opose proof (Lub_Rbar_correct E) as h.
-  rewrite /is_lub_Rbar in h.
+  rewrite /advantage_rbar.
+  set (E := (λ ε0 : R, ∃ (σ σ' : state), nonneg (pr_dist X Y σ σ' v) = ε0)).
+  opose proof (Lub.Lub_Rbar_correct E) as h.
+  rewrite /Lub.is_lub_Rbar in h.
   destruct h as [h1 h2].
   apply h2.
-  rewrite /is_ub_Rbar.
-  intros ε' (σ & σ' & v & hε').
+  rewrite /Lub.is_ub_Rbar.
+  intros ε' (σ & σ' & hε').
   apply rbar_le_rle.
   rewrite -hε'. apply hε.
 Qed.
+
+Lemma advantage_uniform' (X Y : expr) v (ε : R) :
+  (∀ (σ σ' : state), pr_dist X Y σ σ' v <= ε)%R →
+  (advantage X Y v <= ε)%R.
+Proof.
+  intros h.
+  opose proof (advantage_uniform _ _ _ _ h).
+Admitted.
