theories/approxis/examples/security_aux.v
@@ -20,3 +20,87 @@ Fact opt_mult_typed (A : type) : (⊢ᵥ opt_mult : (TOption (TOption A) → TOp
 Proof.
   rewrite /opt_mult. tychk.
 Qed.
+
+
+Definition TList α := (μ: (ref (() + α * #0)))%ty.
+Fact init_list_typed α : ⊢ᵥ init_list : (() → TList α).
+Proof. rewrite /init_list /TList. type_val 1. constructor. tychk. Qed.
+
+Definition TMap k v : type := ref (TList (k * v)).
+Fact init_map_typed k v : ⊢ᵥ init_map : (() → TMap k v).
+Proof. rewrite /init_map /TMap. type_val 1. constructor. tychk.
+       apply init_list_typed.
+Qed.
+
+Definition find_list : val :=
+  (rec: "find" "h" "k" :=
+     match: ! (rec_unfold "h") with
+       NONE => NONE
+     | SOME "p" =>
+         let: "kv" := Fst "p" in
+         let: "next" := Snd "p" in
+         if: (Fst "kv") = "k" then SOME (Snd "kv") else "find" "next" "k"
+     end).
+
+Definition type_closed a := ∀ f, (a = a.[f])%ty.
+
+Fact find_list_typed A B : type_closed A → type_closed B → UnboxedType A → ⊢ᵥ find_list : (TList (A * B) → A → TOption B).
+Proof.
+  intros A_closed B_closed A_unboxed.
+  rewrite /find_list. type_val 1.
+  type_expr 3 ; try by tychk.
+  2: {
+    type_expr 5.
+    2: tychk. 2: tychk.
+    eapply UnboxedEq_typed.
+    1: apply A_unboxed.
+    1,2: tychk.
+  }
+  Unshelve.
+  2: exact TUnit.
+  - set (α := (A * B)%ty).
+    set (unfolded := (ref (() + α * TList α))%ty).
+    assert (unfolded = ((ref (() + α * #0))%ty).[(μ: (ref (() + α * #0)))%ty/]) as ->.
+    { simpl. rewrite /unfolded.
+      rewrite /α /TList.
+      by rewrite -A_closed -B_closed.
+    }
+    eapply TUnfold ; tychk.
+Qed.
+
+Fact get_typed A B :
+  type_closed A → type_closed B → UnboxedType A →
+  ⊢ᵥ get : (TMap A B → A → TOption B)%ty.
+Proof. intros. rewrite /get. tychk. by apply find_list_typed. Qed.
+
+Fact set_typed A B :
+  type_closed A → type_closed B →
+  ⊢ᵥ set : (TMap A B → A → B → TUnit)%ty.
+Proof.
+  intros HA HB.
+  rewrite /set. tychk.
+  rewrite /cons_list. type_val 2.
+  rewrite /TList.
+  constructor.
+  simpl. tychk.
+  simplify_map_eq.
+  f_equal.
+  by rewrite -HA -HB.
+Qed.
+
+
+Fact nat_to_fin_list (MAX : nat) (l:list nat):
+  (∀ x, x ∈ l -> (x < S MAX)%nat) ->
+  ∃ l': (list (fin (S MAX))), fin_to_nat <$> l' = l.
+Proof.
+  clear.
+  induction l as [|a l'].
+  - intros. exists []. naive_solver.
+  - intros. set_unfold.
+    assert (a<S MAX) as H' by naive_solver.
+    unshelve epose proof IHl' _ as [l ?]; first naive_solver.
+    exists (nat_to_fin H'::l).
+    simpl.
+    repeat f_equal; last done.
+    by rewrite fin_to_nat_to_fin.
+Qed.
